#+TITLE: Deriving Rotational Energy
#+AUTHOR: Houjun Liu
#+COURSE: PHYS360
#+SOURCE: KBhPHYS360RotationalKineticEnergy


* Position of $m_i$
In a rigid body consisting of $N$ point masses, the vector to the position of $m_i$ is defined as $\vec{r_i(t)}$, which is defined as follows:

\begin{equation}
    \vec{r_i(t)} = \vec{R_{CM}(t)} + \vec{r_i}'(t)
\end{equation}

whereas, $\vec{R_{CM}(t)}$ is the position vector of the center of mass of the rigid body as a whole, and $\vec{r_i}'(t)$ the vector from the center of mass to $m_i$.

* Velocity of $m_i$
The velocity of $m_i$ is simply determined by the first derivative of the position equation as per above. Namely, that:

\begin{equation}
    \vec{v_i(t)} = \vec{V_{CM}(t)} + \vec{v_i}'(t)
\end{equation}

where, $\vec{v_i(t)}$ is the velocity vector of $m_i$, and $\vec{V_{CM}(t)}$ is the velocity vector of the center of mass of the rigid body, and $\vec{v_i}'(t)$ is the velocity vector from center of mass to $m_i$.

* Deriving $KE_{total}$

** Setting up
From definition of $KE_{total}$ itself, $KE_{total}$ is the sum of all energies of each point mass in the rigid body.

\begin{equation}
    \sum^N_{i=1} \frac{1}{2}m_iv_i^2
\end{equation}


** Derivation, part 1
Expanding this equation and substituting the value of $v_i$, and additionally setting $M = \sum m_i$ (namely, that $M$ represents the total mass of the rigid body) we could derive:

\begin{align}
    \sum^N_{i=1} \frac{1}{2}m_iv_i^2 =& \sum^N_{i=1} \frac{1}{2}m_i(v_i \cdot v_i) \\
    =& \sum^N_{i=1} \frac{1}{2}m_i((\vec{V_{CM}} + \vec{v_i}') \cdot (\vec{V_{CM}} + \vec{v_i}')) \\
    =& \sum^N_{i=1} \frac{1}{2}m_i(\vec{V_{CM}}^2 + 2 \times (\vec{v_i}' \cdot \vec{V_{CM}}) + \vec{v_i}'^2)) \\
    =& \sum^N_{i=1} \frac{1}{2}m_i\vec{V_{CM}}^2 + \sum^N_{i=1} m_i \times (\vec{v_i}' \cdot \vec{V_{CM}}) + \sum^N_{i=1} \frac{1}{2}m_i\vec{v_i}'^2 \\
    =& \frac{1}{2} \vec{V_{CM}}^2 \sum^N_{i=1} m_i + \vec{V_{CM}} \sum^N_{i=1} m_i \vec{v_i}' + \sum^N_{i=1} \frac{1}{2}m_i\vec{v_i}'^2
\end{align}

** Dealing with the Middle Term
At this point, we must note that $\sum^N_{i=1} m_i \vec{v_i}' = 0$. Per the definition of the center of mass, the following holds:

\begin{equation}
    \vec{r_{CM}} = (\frac{1}{M}) \sum_i m_i \vec{r_i}
\end{equation}

Changing reference frame to that of the center of mass itself, this equation therefore becomes:

\begin{equation}
    \vec{r_{CM}}' = (\frac{1}{M}) \sum_i m_i \vec{r_i}'
\end{equation}

It is important to realize here that $\vec{r_{CM}}' = 0$ because of the fact that --- at the reference point of the center of mass, the center of mass is at a zero-vector distance away from itself.

In order to figure a statement with respect to the /velocity/ of $r_i'$, we take the derivative of the previous equation with respect to time.

\begin{align}
    0 =& (\frac{1}{M}) \sum_i m_i \vec{r_i}' \\
    \Rightarrow& \frac{d}{dt} (\frac{1}{M}) \sum_i m_i \vec{r_i}' \\
    =& (\frac{1}{M}) \sum_i m_i \vec{v_i}'
\end{align}

Given that $\frac{1}{M}$ could not be zero for an object with non-zero mass, it is concluded therefore that $\sum_i m_i \vec{v_i}' = 0$.

** Derivation, part 2
As $\sum_i m_i \vec{v_i}' = 0$, the $KE_{total}$ work-in-progress equation's middle term (which contains the statement $\sum_i m_i \vec{v_i}'$) is therefore zero. Substituting that in and removing the term, we therefore result in:

\begin{equation}
     \sum^N_{i=1} \frac{1}{2}m_iv_i^2 = \frac{1}{2} \vec{V_{CM}}^2 \sum^N_{i=1} m_i + \sum^N_{i=1} \frac{1}{2}m_i\vec{v_i}'^2
\end{equation}

Replacing the definition of $M = \sum m_i$, we result in

\begin{align}
     \sum^N_{i=1} \frac{1}{2}m_iv_i^2 &= \frac{1}{2} M \vec{V_{CM}}^2 + \sum^N_{i=1} \frac{1}{2}m_i\vec{v_i}'^2 \\
     KE_{total} &= \frac{1}{2} M \vec{V_{CM}}^2 + \sum^N_{i=1} \frac{1}{2}m_i\vec{v_i}'^2
\end{align}
 
The left term of this equation ($\frac{1}{2} M \vec{V_{CM}}^2$) is the clear original statement for $KE_{translational}$. As component masses of a rigid body cannot experience translational motion about its center of origin, the second term is therefore rotational only and so $KE_{rotational}$. 

Therefore:

\begin{equation}
    KE_{total} = KE_{translational}+KE_{rotational}
\end{equation}

